add semantics duality

Veil/DSL/ActionTheory.lean
@@ -7,11 +7,16 @@ import Veil.DSL.Base
   we use to define initializers and actions.
 -/
 section Veil
-
+open Classical
 /-! ## Types  -/
 section Types
+
+inductive Mode where
+  | internal : Mode
+  | external : Mode
+
 /-! Our language is parametric over the state and return type. -/
-variable (σ ρ : Type)
+variable (m : Mode) (σ ρ : Type)
 
 /-- One-state formula -/
 @[inline] abbrev SProp := σ -> Prop
@@ -27,8 +32,14 @@ variable (σ ρ : Type)
     to a return value `r : ρ` and a post-state `s' : σ`
 -/
 
-/-- Omni semantics, which relates a state `s : σ` to set of the possible program outcomes `post : RProp σ` -/
-abbrev Wlp     := σ -> RProp σ ρ -> Prop
+set_option linter.unusedVariables false in
+/-- Omni semantics, which relates a state `s : σ` to set of the possible program outcomes `post : RProp σ`
+  We have two modes for this monad:
+  - `internal` for function calls. When we call an action, callee should ensure all assertions are satisfied
+    To model that we treat all `require` statements as `assert`'s.
+  - `external` for enviorment calls. In this case envioremnt should provide a necessary conditions to
+    satisfy all `require`'s. To model that we treat all `require` statements as `assume`'s. -/
+abbrev Wlp (m : Mode) (σ ρ : Type) := σ -> RProp σ ρ -> Prop
 /-- [BigStep]: Standard big-step semantics, which relates a state `s : σ` to a return value `r : ρ` and a post-state `s' : σ` -/
 abbrev BigStep := σ -> ρ -> σ -> Prop
 
@@ -53,13 +64,9 @@ variable {σ ρ : Type}
   In theory we could add  ```∀ s, ∃ Q, act s Q``` condition to this definition, but
   this will duplicate the body of `act` twice, increasing the formula which we eventually
   send to the solver.
-
-  Instead, we will add this condition to the `Sound` class, which will allow us to prove
-  the soundness of the `Wlp.toBigStep` conversion for all `Sound` actions. And then we
-  show that all actions we are using in our framework are `Sound`.
    -/
 @[actSimp]
-def Wlp.toBigStep {σ} (act : Wlp σ ρ) : BigStep σ ρ :=
+def Wlp.toBigStep {σ} (act : Wlp m σ ρ) : BigStep σ ρ :=
   fun s r' s' => ¬ act s (fun r₀ s₀ => ¬ (r' = r₀ ∧ s' = s₀))
 
 /-- [BigStep.toWlp] converts Big-step semantics to Omni one.
@@ -67,49 +74,52 @@ def Wlp.toBigStep {σ} (act : Wlp σ ρ) : BigStep σ ρ :=
   Ideally, here we should also assert termination of `act`, but this will be handled
   via `Sound` condition later. -/
 @[actSimp]
-def BigStep.toWlp {σ} (act : BigStep σ ρ) : Wlp σ ρ :=
+def BigStep.toWlp {σ} (act : BigStep σ ρ) : Wlp .internal σ ρ :=
   fun s post => ∀ r s', act s r s' -> post r s'
 
 
 /-- Function which transforms any two-state formula into `Wlp` -/
 @[actSimp]
-def Function.toWlp (r : σ -> σ -> Prop) : Wlp σ Unit :=
+def Function.toWlp (r : σ -> σ -> Prop) : Wlp .internal σ Unit :=
   fun s post => ∀ s', r s s' -> post () s'
 
 /-- Function which transforms any `Wlp` into a two-state formula -/
 @[actSimp]
-def Wlp.toActProp {σ} (act : Wlp σ ρ) : ActProp σ :=
+def Wlp.toActProp {σ} (act : Wlp m σ ρ) : ActProp σ :=
   fun s s' => ¬ act s (fun _ s₀ => ¬ (s' = s₀))
 
 /-! ### Languge statements -/
 
 @[actSimp]
-def Wlp.pure (r : ρ) : Wlp σ ρ := fun s post => post r s
+def Wlp.pure (r : ρ) : Wlp m σ ρ := fun s post => post r s
 @[actSimp]
-def Wlp.bind (wp : Wlp σ ρ) (wp_cont : ρ -> Wlp σ ρ') : Wlp σ ρ' :=
+def Wlp.bind (wp : Wlp m σ ρ) (wp_cont : ρ -> Wlp m σ ρ') : Wlp m σ ρ' :=
   fun s post => wp s (fun r s' => wp_cont r s' post)
 
 @[actSimp]
-def Wlp.assume (rq : Prop) : Wlp σ PUnit := fun s post => rq → post () s
+def Wlp.assume (asm : Prop) : Wlp m σ PUnit := fun s post => asm → post () s
 @[actSimp]
-def Wlp.assert (as : Prop) : Wlp σ PUnit := fun s post => ∀ s', (as -> s = s') -> post () s'
+def Wlp.assert (ast : Prop) : Wlp m σ PUnit := fun s post => ast ∧ post () s
 @[actSimp]
-def Wlp.fresh (τ : Type) : Wlp σ τ := fun s post => ∀ t, post t s
+def Wlp.fresh (τ : Type) : Wlp m σ τ := fun s post => ∀ t, post t s
+
+@[actSimp]
+def Wlp.require (rq : Prop) : Wlp m σ PUnit :=
+  match m with
+  | Mode.internal => Wlp.assert rq
+  | Mode.external => Wlp.assume rq
 
 /-- `Wlp.spec req ens` is the weakest precondition for a function with
   precondition `req` and postcondition `ens`.
-  The intuition begind this definition is:
-  - if `req s` holds in a current state `s`, then we it is equivalent to
-    `∀ r' s', ens s r' s' -> post r' s'`, meaning that, we have to prove
-    `post`, assuming that `ens` holds.
-  - if `req s` does not hold, then we do not know anything about the behiavor
-    of the function i.e. it can execute to any post-state `s'` and return any
-    value `r'`. Hence we have to show `post` for all possible return values.
-    `Wlp.spec` in this case is equivalent to `∀ r' s', post r' s'`.
 -/
 @[actSimp]
-def Wlp.spec (req : SProp σ) (ens : σ -> RProp σ ρ) : Wlp σ ρ :=
-  fun s post => ∀ r' s', (req s -> ens s r' s') -> post r' s'
+def Wlp.spec (req : SProp σ) (ens : σ -> RProp σ ρ) : Wlp m σ ρ :=
+  fun s post =>
+    match m with
+    | .internal => req s ∧ ∀ r' s', (ens s r' s' -> post r' s')
+    | .external => ∀ r' s', req s -> ens s r' s' -> post r' s'
+
+
 
 def BigStep.spec (req : SProp σ) (ens : σ -> RProp σ ρ) : BigStep σ ρ :=
   fun s r s' => req s -> ens s r s'
@@ -126,11 +136,11 @@ def BigStep.spec (req : SProp σ) (ens : σ -> RProp σ ρ) : BigStep σ ρ :=
 
 /-! ### Monad Instances -/
 
-instance : Monad (Wlp σ) where
+instance : Monad (Wlp m σ) where
   pure := Wlp.pure
   bind := Wlp.bind
 
-instance : MonadStateOf σ (Wlp σ) where
+instance : MonadStateOf σ (Wlp m σ) where
   get := fun s post => post s s
   set s' := fun _ post => post () s'
   modifyGet := fun act s post => let (ret, s') := act s ; post ret s'
@@ -140,10 +150,23 @@ class IsStateExtension (σ : semiOutParam Type) (σ' : Type) where
   restrictTo : σ' -> σ
 
 export IsStateExtension (extendWith restrictTo)
-instance [IsStateExtension σ σ'] : MonadLift (Wlp σ) (Wlp σ') where
+instance [IsStateExtension σ σ'] : MonadLift (Wlp m σ) (Wlp m σ') where
   monadLift := fun m s post => m (restrictTo s) (fun r s' => post r (extendWith s' s))
 
 /-! ### Soundness proof -/
+
+abbrev refines {σ ρ} (act : Wlp m σ ρ) (act' : Wlp m σ ρ) : Prop :=
+  ∀ s post, act s post -> act' s post
+
+instance : LE (Wlp m σ ρ) where
+  le := refines
+
+abbrev Wlp.triple {σ ρ} (req : SProp σ) (act : Wlp m σ ρ) (ens : RProp σ ρ) : Prop :=
+  ∀ s, req s -> act s ens
+
+abbrev ActProp.triple {σ } (req : SProp σ) (act : ActProp σ) (ens : SProp σ) : Prop :=
+  ∀ s s', req s -> act s s' -> ens s'
+
 
 /-- `Sound act` states the set of minimal conditions on `act` that are required
   to prove the soundness of the `Wlp.toBigStep` conversion.
@@ -158,137 +181,167 @@ instance [IsStateExtension σ σ'] : MonadLift (Wlp σ) (Wlp σ') where
     predicates `post`
   - second condition `impl`, states that we can always weaken the postcondition of `act`
     by adding some of the possible outcomes.
-
-  Note that, as captured by `sound_terminates`, the `Sound act` ensures that `act`
-  terminates.
--/
-class Sound {σ ρ : Type} (act : Wlp σ ρ) where
-  inter {τ : Type} (post : τ -> RProp σ ρ) :
-    ∀ s : σ, (∀ t : τ, act s (post t)) -> act s (∀ t, post t · ·)
+  - third condition `call`, states that the `internal` mode of `act` refines the `external`
+    one. In other words, if you have proven some striple for `internal` mode of `act`,
+    the same one holds for its `external` version -/
+class Sound {σ ρ : Type} (act : (m : Mode) -> Wlp m σ ρ) where
+  inter {m} {τ : Type} [Inhabited τ] (post : τ -> RProp σ ρ) :
+    ∀ s : σ, (∀ t : τ, act m s (post t)) -> act m s (∀ t, post t · ·)
   impl (post post' : RProp σ ρ) : ∀ s,
-    (∀ r s, post r s -> post' r s) -> act s post -> act s post'
+    (∀ r s, post r s -> post' r s) -> act m s post -> act m s post'
+  call : act .internal <= act .external
 
-theorem sound_and (act : Wlp σ ρ) [Sound act] :
-  act s post -> act s post' -> act s fun r s => post r s ∧ post' r s := by
+theorem sound_and (act : ∀ m, Wlp m σ ρ) [Sound act] :
+  act m s post -> act m s post' -> act m s fun r s => post r s ∧ post' r s := by
   intro hact hact'
   let Post := fun (b : Bool) => if b then post' else post
   have post_eq : (fun r s => ∀ b, Post b r s) = fun r s => post r s ∧ post' r s := by
     unfold Post; simp
   rw [<-post_eq]; apply Sound.inter <;> simp [*, Post]
 
-theorem sound_terminates [Sound act] : (∀ r s, post r s) -> act s post := by
-  intro hpost
-  have post_eq : post = (fun _ _ => Empty -> True) := by ext; simp_all
-  rw [post_eq]; apply Sound.inter; rintro ⟨⟩
+-- theorem sound_terminates [Sound act] : (∀ r s, post r s) -> act m s post := by
+--   intro hpost
+--   have post_eq : post = (fun _ _ => Empty -> True) := by ext; simp_all
+--   rw [post_eq]; apply Sound.inter; rintro ⟨⟩
 
-theorem wlp_sound (act : Wlp σ ρ) [Sound act] :
-  ∀ s post, act.toBigStep.toWlp s post <-> act s post := by
-  intro s post; constructor
-  { unfold Wlp.toBigStep BigStep.toWlp; simp
-    intro hact
-    have post_impl : ∀ r s, (∀ r' s', ¬ post r' s' -> ¬ (r' = r ∧ s' = s)) -> post r s := by
-      intro r s impl
-      false_or_by_contra
-      specialize impl r s; apply impl <;> simp_all
-    apply Sound.impl; apply post_impl
-    apply Sound.inter; intro r'
-    apply Sound.inter; intro s'
-    by_cases postrs : post r' s'
-    { apply sound_terminates; simp_all }
-    apply Sound.impl (post := fun r₀ s₀ => r' = r₀ → ¬s' = s₀) <;> simp_all
-    false_or_by_contra
-    specialize hact _ _ ‹_›; contradiction }
-  intro hact r' s' h
-  false_or_by_contra; apply h; apply Sound.impl (post := post)
-  { intros; intro _; simp_all }
-  assumption
+-- theorem wlp_sound (act : ∀ m, Wlp m σ ρ) [Sound act] :
+--   ∀ s post, (act m).toBigStep.toWlp (m := m) s post <-> act m s post := by
+--   intro s post; constructor
+--   { unfold Wlp.toBigStep BigStep.toWlp; simp
+--     intro hact
+--     have post_impl : ∀ r s, (∀ r' s', ¬ post r' s' -> ¬ (r' = r ∧ s' = s)) -> post r s := by
+--       intro r s impl
+--       false_or_by_contra
+--       specialize impl r s; apply impl <;> simp_all
+--     apply Sound.impl; apply post_impl
+--     apply Sound.inter; intro r'
+--     apply Sound.inter; intro s'
+--     by_cases postrs : post r' s'
+--     { apply sound_terminates; simp_all }
+--     apply Sound.impl (post := fun r₀ s₀ => r' = r₀ → ¬s' = s₀) <;> simp_all
+--     false_or_by_contra
+--     specialize hact _ _ ‹_›; contradiction }
+--   intro hact r' s' h
+--   false_or_by_contra; apply h; apply Sound.impl (post := post)
+--   { intros; intro _; simp_all }
+--   assumption
 
 theorem triple_sound [Sound act] (req : SProp σ) (ens : SProp σ) :
-  (∀ s s', req s -> act.toActProp s s' -> ens s') ->
-  ∀ s, req s -> act s (fun _ => ens) := by
-  intro htriple s hreq
-  have ens_impl : ∀ s, (∀ s', ¬ ens s' -> ¬ (s' = s)) -> ens s := by
-    intro s impl
+  (¬ ∀ s, ens s) ->
+  (act m).toActProp.triple req ens -> (act m).triple req (fun _ => ens) := by
+  intro ensTaut htriple s hreq
+  have ens_impl : ∀ s, (∀ s' : { s' // ¬ ens s' }, ¬ (s'.val = s)) -> ens s := by
+    simp; intro s impl
     false_or_by_contra
     specialize impl s; apply impl <;> simp_all
   apply Sound.impl; intro _; apply ens_impl
-  apply Sound.inter; intro s'
-  by_cases hens : ens s'
-  { apply sound_terminates; simp_all }
+  simp at ensTaut; rcases ensTaut with ⟨s', hens⟩
+  have: Inhabited { s' // ¬ ens s' } := ⟨⟨_, hens⟩⟩
+  apply Sound.inter; rintro ⟨s', hens⟩
   apply Sound.impl (post := fun r₀ s₀ => ¬s' = s₀) <;> (intros; try simp_all)
   false_or_by_contra
   specialize htriple _ _ ‹_› ‹_›; contradiction
 
-instance : Sound (Wlp.pure (σ := σ) r) where
+instance : Sound (Wlp.pure (m := ·) (σ := σ) r) where
   inter := by simp [actSimp]
-  impl := by intros; simp_all [actSimp]
+  impl  := by intros; simp_all [actSimp]
+  call  := by solve_by_elim
 
-instance [Sound act] [∀ r, Sound (act' r)] : Sound (Wlp.bind act act') where
+instance (act' : ρ -> ∀ m, Wlp m σ ρ) [Sound act] [∀ r, Sound (act' r)] : Sound (fun m => Wlp.bind (act m) (act' · m)) where
   inter := by
     unfold Wlp.bind
-    intros τ post s hbind
-    apply Sound.impl (∀ t, act' · · <| post t) <;> solve_by_elim [Sound.inter]
+    intros m τ _ post s hbind
+    apply Sound.impl (∀ t, act' · m · <| post t) <;> solve_by_elim [Sound.inter]
   impl := by
     unfold Wlp.bind
-    intros post post' s hpost hbind
-    apply Sound.impl (act' · · <| post) <;> (intros; solve_by_elim [Sound.impl])
+    intros m post post' s hpost hbind
+    apply Sound.impl (act' · m · <| post) <;> (intros; solve_by_elim [Sound.impl])
+  call := by
+    unfold Wlp.bind
+    intros s post hbind
+    apply Sound.call; apply Sound.impl;
+    { intros _ _; apply Sound.call }
+    solve_by_elim
 
-instance : Sound (Wlp.assume (σ := σ) rq) where
+instance : Sound (Wlp.assume (m := ·) (σ := σ) rq) where
   inter := by intros; simp_all [actSimp]
   impl := by intros; simp_all [actSimp]
+  call := by solve_by_elim
 
-instance : Sound (Wlp.assert (σ := σ) rq) where
-  inter := by intros; simp_all [actSimp]
-  impl := by intros; simp_all [actSimp] <;> solve_by_elim
+instance : Sound (Wlp.assert (m := ·) (σ := σ) rq) where
+  inter := by intros; simp_all [actSimp]; rename_i h; specialize h default; simp [*]
+  impl  := by intros; simp_all [actSimp] <;> solve_by_elim
+  call  := by solve_by_elim
 
-instance : Sound (Wlp.fresh (σ := σ) τ) where
+instance : Sound (Wlp.require (m := ·) (σ := σ) rq) where
+  inter := by
+    intros m; cases m
+    { intros; simp_all [actSimp]; rename_i h; specialize h default; simp [*] }
+    intros; simp_all [actSimp]
+  impl := by intros m; cases m <;> (intros; simp_all [actSimp] <;> solve_by_elim)
+  call := by
+   intros s post; unfold Wlp.require; simp [Wlp.assert, Wlp.assume]; solve_by_elim
+
+
+instance : Sound (Wlp.fresh (m := ·) (σ := σ) τ) where
   inter := by intros; simp_all [actSimp]
   impl := by intros; simp_all [actSimp]
+  call := by solve_by_elim
 
-instance : Sound (Wlp.spec req ens) where
-  inter := by intros; simp_all [actSimp]
-  impl := by simp [actSimp]; intros; solve_by_elim
 
-instance (r : σ -> σ -> Prop) : Sound (r.toWlp) where
+instance : Sound (Wlp.spec (m := ·) req ens) where
+  inter := by
+    intro m; cases m <;> (intros; simp_all [actSimp])
+    rename_i h; intros; specialize h default; simp [*]
+  impl := by
+    intro m; cases m <;> (simp [actSimp]; intros)
+    { constructor <;> (intros; solve_by_elim) }
+    solve_by_elim
+  call := by intros _; simp_all [actSimp]
+
+instance (r : σ -> σ -> Prop) : Sound (fun _ => r.toWlp) where
   inter := by intros; simp_all [actSimp]
   impl := by intros; simp_all [actSimp]
+  call := by solve_by_elim
 
-instance : Sound (get (σ := σ)) where
+instance : Sound (get (m := Wlp · σ)) where
   inter := by intros; simp_all [get, getThe,MonadStateOf.get]
   impl := by intros; simp_all [get, getThe,MonadStateOf.get]
+  call := by solve_by_elim
 
-instance (s : σ) : Sound (set s : Wlp σ PUnit) where
+instance (s : σ) : Sound (set s (m := Wlp · σ)) where
   inter := by intros; simp_all [set,MonadStateOf.set]
   impl := by intros; simp_all [set,MonadStateOf.set]
+  call := by solve_by_elim
 
-instance : Sound (modifyGet (σ := σ) f) where
+instance : Sound (modifyGet f (m := Wlp · σ)) where
   inter := by intros; simp_all [modifyGet,MonadStateOf.modifyGet]
   impl := by intros; simp_all [modifyGet,MonadStateOf.modifyGet]
+  call := by solve_by_elim
 
-instance (act : Wlp σ ρ) [IsStateExtension σ σ'] [Sound act] :
-  Sound (monadLift act : Wlp σ' ρ) where
+instance (act : ∀ m, Wlp m σ ρ) [IsStateExtension σ σ'] [Sound act] :
+  Sound (fun m => monadLift (m := Wlp m σ) (n := Wlp m σ') (act m)) where
   inter := by
     intros; simp_all [monadLift, MonadLift.monadLift]
     solve_by_elim [Sound.inter]
   impl := by
     intros; simp_all [monadLift, MonadLift.monadLift]
     solve_by_elim [Sound.impl]
+  call := by
+    intros; simp_all [monadLift, MonadLift.monadLift]
+    solve_by_elim [Sound.call]
 
 /-! ### Correctness of `checkSpec` -/
 
 theorem wlp_spec_to_big_step :
-  (Wlp.spec ens req).toBigStep = BigStep.spec ens req := by
+  (Wlp.spec ens req).toBigStep (m := .internal) = BigStep.spec ens req := by
   ext s r' s'; unfold Wlp.spec BigStep.spec Wlp.toBigStep; simp
 
 theorem check_spec_sound [Sound act] (req : SProp σ) (ens : σ -> RProp σ ρ) :
-  (∀ s, req s -> act s (ens s)) ->
-  (∀ s post, Wlp.spec req ens s post -> act s post) := by
-  intro triple s post hspec
-  apply Sound.impl; apply hspec
-  have: ∀ r' s', ({t : Unit // req s} → ens s r' s') ->  (req s → ens s r' s') := by
-    intro r' s' h hreq; apply h; exact ⟨(), hreq⟩
-  apply Sound.impl; apply this
-  apply Sound.inter; rintro ⟨_, hreq⟩
-  solve_by_elim
+  (∀ s, req s -> act m s (ens s)) ->
+  Wlp.spec (m := .internal) req ens <= act m := by
+  intro triple s post; simp [actSimp]; intros hreq hens
+  solve_by_elim [Sound.impl]
+
 
 end Theory
