Test/InternalExternal.lean
@@ -1,0 +1,16 @@
+import Veil.DSL
+import Veil.TestUtil
+
+namespace Test
+open Classical
+
+individual x : Prop
+
+#gen_state
+
+action req = {
+  require False
+}
+
+example : forall s s' (Q : Prop), req.tr s s' -> Q := by simp [actSimp]
+example : forall s Q, ¬ req s Q := by simp [actSimp]
