Test/NonDetAssn.lean
@@ -16,7 +16,7 @@ action nondet_individual = {
 
 /--
 info: def Test.nondet_individual : {node : Type} →
-  [node_dec : DecidableEq node] → [node_ne : Nonempty node] → Wlp (State node) PUnit :=
+  [node_dec : DecidableEq node] → [node_ne : Nonempty node] → Wlp Mode.internal (State node) PUnit :=
 fun {node} [DecidableEq node] [Nonempty node] =>
   let t := fun s post => ∀ (t : Prop), post PUnit.unit { x := t, r := s.r };
   t
@@ -31,7 +31,7 @@ action quantify_fresh (n : node) = {
 
 /--
 info: def Test.quantify_fresh : {node : Type} →
-  [node_dec : DecidableEq node] → [node_ne : Nonempty node] → node → Wlp (State node) PUnit :=
+  [node_dec : DecidableEq node] → [node_ne : Nonempty node] → node → Wlp Mode.internal (State node) PUnit :=
 fun {node} [DecidableEq node] [Nonempty node] n =>
   let t := fun s post =>
     ∀ (t : node → node → Prop), post PUnit.unit { x := s.x, r := fun x N => if x = n then t n N else s.r x N };
@@ -46,7 +46,7 @@ action double_quant = {
 
 /--
 info: def Test.double_quant : {node : Type} →
-  [node_dec : DecidableEq node] → [node_ne : Nonempty node] → Wlp (State node) PUnit :=
+  [node_dec : DecidableEq node] → [node_ne : Nonempty node] → Wlp Mode.internal (State node) PUnit :=
 fun {node} [DecidableEq node] [Nonempty node] =>
   let t := fun s post =>
     ∀ (t : node → node → Prop), post PUnit.unit { x := s.x, r := fun N x => if x = N then t N N else s.r N x };
